update

sigma.v
@@ -1,33 +1,62 @@
 Require Import Program Arith ZArith Lia.
-
-  
  (* Program Fixpoint solution_1 (f: Z -> Z) (a b: Z) {measure (Z.to_nat (b-a + 1))}: Z :=
   if Z.ltb b a then 0
   else if Z.eqb a b then f a
   else f a + solution_1 f (a + 1) b.
 
   Next Obligation.
-  Proof. *)
-    
+  Proof. 
+    intros.
+    apply Z2Nat.inj_lt.
+    Open Scope Z_scope.
+    -   *)
+  
+ Program Fixpoint solution_1 (f: nat -> nat) (a b: nat) {measure (b - a)}: nat :=
+  match b - a with
+  | 0 => f a
+  | _ => f a + solution_1 f (a+1) b
+  end.
+
+  Next Obligation.
+  Proof. 
+     auto with *.
+    Qed.
 
 
-Program Fixpoint solution_2 (f: nat -> nat) (a b : nat) {measure (b-a)} : nat :=
+(* Program Fixpoint solution_2 (f: nat -> nat) (a b : nat) {measure (b-a)} : nat :=
     if (Nat.ltb b a) then 0 
     else (f b) + solution_2 f a (b-1).
-  
+  *)
 
-Program Fixpoint solution_2 (f: nat -> nat) (a: nat) (b : nat) : nat :=
-    ,match b - a with
+Program Fixpoint solution_2 (f: nat -> nat) (a: nat) (b : nat) {measure (b - a)}: nat :=
+    match b - a with
     | 0 => f b
     | _ => f b + solution_2 f a (b-1)
     end.
 Next Obligation.
 Proof.
-    specialize (solution_2 f a (b-1)).
-    apply solution_2.
+    auto with *.
+Qed.
 
-    
-.
+Theorem eq: forall f a b, a <= b -> solution_1 f a b = solution_2 f a b.
+Proof.
+    intro f.
+    intros.
+    pose (c := b - a).
+    assert (H1: b = a + c).
+    { 
+        unfold c.
+        assert (H2:= Nat.add_sub_assoc).
+        specialize H2 with a b a.
+        rewrite H2.
+        assert (H3:= Nat.add_sub_swap).
+        specialize H3 with a b a.
+        rewrite H3.
+        lia.
+        lia.
+        apply H.
+     }
+
 
 Program Fixpoint aux (a:nat) (b:nat) (f:nat->nat) (acc:nat) : nat :=
 if (Nat.ltb b a) then acc else aux (a+1) b f (acc + (f a))
